src/PushButtonSynthesis/BaseConversion.v
@@ -63,6 +63,18 @@ Local Opaque
       reified_convert_bases_gen
       expr.Interp.
 
+Inductive bounds := exactly (_ : list Z) | use_prime | use_bitwidth.
+
+Global Instance show_bounds : Show bounds
+  := fun with_parens v
+     => match v with
+        | use_prime => "use_prime"
+        | use_bitwidth => "use_bitwidth"
+        | exactly l => @show_list _ PowersOfTwo.show_Z with_parens l
+        end%string.
+
+Definition default_bounds : bounds := use_prime.
+
 Section __.
   Context {output_language_api : ToString.OutputLanguageAPI}
           {static : static_opt}
@@ -72,12 +84,15 @@ Section __.
           {should_split_mul : should_split_mul_opt}
           {widen_carry : widen_carry_opt}
           {widen_bytes : widen_bytes_opt}
+          (s : Z) (c : list (Z * Z))
           (src_n : nat)
           (src_limbwidth : Q)
           (dst_limbwidth : Q)
           (machine_wordsize : Z)
-          (max_opt : option Z)
-          (inbounds_multiplier : option Q).
+          (inbounds_multiplier : option Q)
+          (outbounds_multiplier : option Q)
+          (inbounds : bounds)
+          (outbounds : bounds).
 
   Local Notation src_weight := (weight (Qnum src_limbwidth) (Qden src_limbwidth)).
   Local Notation dst_weight := (weight (Qnum dst_limbwidth) (Qden dst_limbwidth)).
@@ -85,21 +100,35 @@ Section __.
   Local Notation force_power_of_two v
     := (2^Z.log2_up v) (only parsing).
 
-  Let max : Z
-    := force_power_of_two
-         (Option.value
-            max_opt
-            (src_weight src_n)).
-
-  Let dst_n : nat
-    := Z.to_nat (Qceiling (Z.log2_up max / dst_limbwidth)).
-
   Let in_upperbounds : list Z
     := List.map
          (fun v : Z => Qceiling (Option.value inbounds_multiplier 1 * v))
-         (encode_no_reduce src_weight src_n (max - 1)).
+         (let encode := encode_no_reduce src_weight src_n in
+          match inbounds with
+          | exactly l => l
+          | use_prime => encode (s - 1)
+          | use_bitwidth => encode (src_weight src_n - 1)
+          end).
+  Let dst_n : nat
+    := let max := match outbounds with
+                  | exactly l => inl (List.length l)
+                  | use_prime => inr s
+                  | use_bitwidth => inr (src_weight src_n)
+                  end in
+       match max with
+       | inl len => len
+       | inr max
+         => Z.to_nat (Qceiling (Z.log2_up max / dst_limbwidth))
+       end.
   Let out_upperbounds : list Z
-    := (encode_no_reduce dst_weight dst_n (max - 1)).
+    := List.map
+         (fun v : Z => Qceiling (Option.value outbounds_multiplier 1 * v))
+         (let encode := encode_no_reduce dst_weight dst_n in
+          match outbounds with
+          | exactly l => l
+          | use_prime => encode (s - 1)
+          | use_bitwidth => encode (dst_weight dst_n - 1)
+          end).
 
   (* We include [0], so that even after bounds relaxation, we can
        notice where the constant 0s are, and remove them. *)
@@ -114,92 +143,6 @@ Section __.
 
   Local Instance split_mul_to : split_mul_to_opt := split_mul_to_of_should_split_mul machine_wordsize possible_values_of_machine_wordsize_with_bytes.
 
-  Lemma length_in_upperbounds : List.length in_upperbounds = src_n.
-  Proof using Type. cbv [in_upperbounds]; now autorewrite with distr_length. Qed.
-  Hint Rewrite length_in_upperbounds : distr_length.
-  Lemma length_out_upperbounds : List.length out_upperbounds = dst_n.
-  Proof using Type. cbv [out_upperbounds]; now autorewrite with distr_length. Qed.
-  Hint Rewrite length_out_upperbounds : distr_length.
-  Lemma length_in_bounds : List.length in_bounds = src_n.
-  Proof using Type. cbv [in_bounds]; now autorewrite with distr_length. Qed.
-  Hint Rewrite length_in_bounds : distr_length.
-  Lemma length_out_bounds : List.length out_bounds = dst_n.
-  Proof using Type. cbv [out_bounds]; now autorewrite with distr_length. Qed.
-  Hint Rewrite length_out_bounds : distr_length.
-
-  Lemma max_None_le_weight : (1 <= src_limbwidth)%Q -> src_n <> 0%nat -> max_opt = None -> 1 < max <= src_weight src_n.
-  Proof using Type.
-    clear.
-    cbv [max Option.value weight Qle]; cbn [Qnum Qden]; autorewrite with zsimplify_const;
-      intros; subst.
-    rewrite !Z.log2_up_pow2 by (Z.div_mod_to_quot_rem; nia).
-    rewrite <- Z.pow_gt_1 by lia.
-    split; [ | lia ]; Z.div_mod_to_quot_rem; nia.
-  Qed.
-
-  Lemma max_Some_le_weight (v := Option.value max_opt 0) : max_opt = Some v -> (1 <= src_limbwidth)%Q -> 1 < v <= src_weight src_n -> 1 < max <= src_weight src_n.
-  Proof using Type.
-    clear.
-    clearbody v.
-    intro; cbv [max Option.value weight Qle]; cbn [Qnum Qden]; subst max_opt.
-    intros; rewrite <- Z.pow_gt_1 by lia; destruct_head'_and.
-    split; auto using Z.log2_up_pos with lia; [].
-    Z.peel_le.
-    etransitivity; [ apply Z.log2_up_le_mono; eassumption | ].
-    rewrite Z.log2_up_pow2; [ reflexivity | ].
-    Z.div_mod_to_quot_rem;
-      repeat match goal with
-             | [ H : context[- ?v] |- _ ]
-               => is_var v; assert (v <= 0) by nia; Z.replace_with_neg v
-             | [ |- context[- ?v] ]
-               => is_var v; assert (v <= 0) by nia; Z.replace_with_neg v
-             end;
-      nia.
-  Qed.
-
-  Lemma dst_weight_n_ge_max : (1 <= dst_limbwidth)%Q -> max <= dst_weight dst_n.
-  Proof using Type.
-    clear.
-    assert (0 <= Z.log2_up max) by auto with zarith.
-    cbv [dst_n weight].
-    cbv [inject_Z Qceiling Qfloor Qdiv Qmult Qopp Qinv Qle Pos.mul Qnum Qden];
-      break_innermost_match; autorewrite with zsimplify_const;
-        try lia.
-    intros; eapply Z.le_trans; [ apply Z.log2_up_le_full | Z.peel_le ].
-    rewrite !Z2Nat.id;
-      Z.div_mod_to_quot_rem;
-      repeat match goal with
-             | [ H : context[- ?v] |- _ ]
-               => is_var v; assert (v <= 0) by nia; Z.replace_with_neg v
-             | [ |- context[- ?v] ]
-               => is_var v; assert (v <= 0) by nia; Z.replace_with_neg v
-             end;
-      nia.
-  Qed.
-
-  Lemma dst_n_nz : 1 < max -> (1 <= dst_limbwidth)%Q -> dst_n <> 0%nat.
-  Proof using Type.
-    clear.
-    intro; assert (0 < Z.log2_up max) by auto using Z.log2_up_pos.
-    subst dst_n.
-    cbv [inject_Z Qceiling Qfloor Qdiv Qmult Qopp Qinv Qle Pos.mul Qnum Qden];
-      break_innermost_match; autorewrite with zsimplify_const;
-        try lia.
-    rewrite <- Z2Nat.inj_0.
-    intros; Z.div_mod_to_quot_rem.
-    repeat match goal with
-           | [ H : context[- ?v] |- _ ]
-             => is_var v; assert (v < 0) by nia; Z.replace_with_neg v
-           | [ |- context[- ?v] ]
-             => is_var v; assert (v < 0) by nia; Z.replace_with_neg v
-           end.
-    rewrite Z2Nat.inj_iff by nia; nia.
-  Qed.
-
-  Local Notation dummy_not_zero_nat := (1%nat) (only parsing).
-  Local Notation dummy_gt_1_Z := (2%Z) (only parsing).
-  Local Notation dummy_le_weight_Z := (-1%Z) (only parsing).
-
   (** Note: If you change the name or type signature of this
         function, you will need to update the code in CLI.v *)
   Definition check_args {T} (res : Pipeline.ErrorT T)
@@ -210,12 +153,13 @@ Section __.
          [(negb (Qle_bool 1 src_limbwidth)%Q, Pipeline.Value_not_leQ "src_limbwidth < 1" 1%Q src_limbwidth);
             (negb (Qle_bool 1 dst_limbwidth)%Q, Pipeline.Value_not_leQ "dst_limbwidth < 1" 1%Q dst_limbwidth);
             ((src_n =? 0)%nat, Pipeline.Values_not_provably_distinctZ "src_n = 0" src_n 0%nat);
-            (let max := Option.value max_opt dummy_gt_1_Z in
-             (negb (1 <? max)%Z,
-              Pipeline.Value_not_ltZ "max ≤ 1" 1 max));
-            (let max := Option.value max_opt dummy_le_weight_Z in
-             (negb (max <=? src_weight src_n)%Z,
-              Pipeline.Value_not_leZ "src_weight src_n < max" max (src_weight src_n)));
+            ((dst_n =? 0)%nat, Pipeline.Values_not_provably_distinctZ "dst_n = 0" dst_n 0%nat);
+            (negb (List.length in_bounds =? src_n)%nat, Pipeline.Values_not_provably_equalZ "length in_bounds ≠ src_n" (List.length in_bounds) src_n);
+            (negb (List.length in_upperbounds =? src_n)%nat, Pipeline.Values_not_provably_equalZ "length in_upperbounds ≠ src_n" (List.length in_upperbounds) src_n);
+            (negb (List.length out_bounds =? dst_n)%nat, Pipeline.Values_not_provably_equalZ "length out_bounds ≠ dst_n" (List.length out_bounds) dst_n);
+            (negb (List.length out_upperbounds =? dst_n)%nat, Pipeline.Values_not_provably_equalZ "length out_upperbounds ≠ dst_n" (List.length out_upperbounds) dst_n);
+            ((negb (Associational.eval c <? s))%Z, Pipeline.Value_not_ltZ "s ≤ Associational.eval c" (Associational.eval c) s);
+            ((s =? 0)%Z, Pipeline.Values_not_provably_distinctZ "s = 0" s 0);
             (let eval_in_upperbounds := eval src_weight src_n in_upperbounds in
              let dst_weight_n := dst_weight dst_n in
              (negb (eval_in_upperbounds <? dst_weight_n)%Z,
@@ -248,10 +192,25 @@ Section __.
                  | solve [ auto ]
                  | progress break_innermost_match_hyps ].
 
+  Ltac prepare_use_curve_good _ :=
+    let curve_good := lazymatch goal with | curve_good : check_args _ = Success _ |- _ => curve_good end in
+    clear -curve_good;
+    cbv [check_args fold_right] in curve_good |- *;
+    repeat first [ match goal with
+                   | [ H : context[match ?b with true => _ | false => _ end ] |- _ ] => destruct b eqn:?
+                   end
+                 | discriminate
+                 | progress Reflect.reflect_hyps
+                 | assumption
+                 | apply conj
+                 | progress destruct_head'_and ].
+
   Context (curve_good : check_args (Success tt) = Success tt).
 
   Lemma use_curve_good
     : 0 < machine_wordsize
+      /\ s - Associational.eval c <> 0
+      /\ s <> 0
       /\ src_n <> 0%nat
       /\ dst_n <> 0%nat
       /\ List.length in_bounds = src_n
@@ -260,37 +219,9 @@ Section __.
       /\ List.length out_upperbounds = dst_n
       /\ 0 < Qden src_limbwidth <= Qnum src_limbwidth
       /\ 0 < Qden dst_limbwidth <= Qnum dst_limbwidth
-      /\ 1 < max <= src_weight src_n
-      /\ 1 < max <= dst_weight dst_n
       /\ eval src_weight src_n in_upperbounds < dst_weight dst_n.
   Proof using curve_good.
-    clear -curve_good.
-    pose proof max_None_le_weight.
-    pose proof dst_weight_n_ge_max.
-    pose proof dst_n_nz.
-    pose proof max_Some_le_weight.
-    cbv [check_args fold_right] in curve_good |- *.
-    autorewrite with distr_length.
-    break_innermost_match_hyps; try discriminate.
-    rewrite negb_false_iff in *.
-    Z.ltb_to_lt.
-    rewrite Qle_bool_iff in *.
-    rewrite NPeano.Nat.eqb_neq in *.
-    cbv [Option.value] in *.
-    cbv [Qnum Qden limbwidth Qceiling Qfloor Qopp Qdiv Qplus inject_Z Qmult Qinv] in *.
-    specialize_by_assumption.
-    repeat apply conj.
-    { use_curve_good_t. }
-    { use_curve_good_t. }
-    { use_curve_good_t. }
-    { use_curve_good_t. }
-    { use_curve_good_t. }
-    { use_curve_good_t. }
-    { use_curve_good_t. }
-    { use_curve_good_t. }
-    { use_curve_good_t. }
-    { use_curve_good_t. }
-    { use_curve_good_t. }
+    prepare_use_curve_good ().
     { use_curve_good_t. }
     { use_curve_good_t. }
     { use_curve_good_t. }
@@ -311,7 +242,9 @@ Section __.
                 dst_weightf "dst_weight"
                 (CorrectnessStringification.dyn_context.cons
                    dst_evalf "dst_eval"
-                   CorrectnessStringification.dyn_context.nil))))%string.
+                   (CorrectnessStringification.dyn_context.cons
+                      (s - Associational.eval c) "(s - c)"
+                      CorrectnessStringification.dyn_context.nil)))))%string.
   Local Notation "'docstring_with_summary_from_lemma!' summary correctness"
     := (docstring_with_summary_from_lemma_with_ctx!
           notations_for_docstring
@@ -374,6 +307,8 @@ Section __.
                       | lia
                       | match goal with
                         | [ H : context[List.map (fun _ => 0) _] |- _ ] => erewrite <- zeros_ext_map, ?eval_zeros in H by reflexivity
+                        | [ H : List.length ?l = ?n, H' : context[eval ?w ?n (zeros (List.length ?l))] |- _ ]
+                          => rewrite !H, eval_zeros in H'
                         end
                       | progress autorewrite with distr_length push_eval in *
                       | destruct_head'_and; eapply Z.le_lt_trans; eassumption ].
@@ -404,8 +339,7 @@ Section __.
               ++ [""]
               ++ (ToString.comment_block
                     ["Computed values:";
-                       "dst_n = " ++ show false dst_n;
-                       "max = " ++ PowersOfTwo.show_Z false max]%string)
+                       "dst_n = " ++ show false dst_n]%string)
               ++ [""])
            function_name_prefix requests.
   End for_stringification.
